wip on eval

concrete/eval.v
@@ -12,7 +12,6 @@ Open Scope Z_scope.
 
 Section WithClasses.
 
-
 Context (mt : machine_types).
 Context {ops : machine_ops mt}.
 
@@ -38,10 +37,15 @@ Let patom := atom pvalue pvalue.
 
 Let atom := atom (word mt) (word mt).
 
-Definition known  (pv:pvalue): option (word mt)  :=
+Fixpoint known  (pv:pvalue): option (word mt)  :=
 match pv with
 | C a => Some a
-| _ => None  (* could try to be smarter if it proves useful *)
+| E f a b =>  (* not clear whether this makes any difference *)
+    match known a,known b with
+    | Some a', Some b' => Some (binop_denote f a' b')
+    | _,_ => None
+    end
+| _ => None  
 end.
 
 Local Notation memory := (word_map mt patom).
@@ -56,7 +60,10 @@ Record pstate := mkPState {
   pepc   : patom
 }.
 
+
 Inductive tstate :=
+| Halted : tstate
+| UnknownUserSt : tstate 
 | St : pstate -> tstate
 | Ch : pvalue (* Zero? *) -> tstate -> tstate -> tstate.
 
@@ -90,35 +97,39 @@ Definition add_rule (cache : rules) (masks: Masks) (mem : memory) : option rules
          @mkRVec pvalue (val atrpc) (val atr)) :: cache).
 
 (* For now, we assume that our parametric machine is always
-running with pc tag = Kernel, and that its own cache lookups
-behave like the ground rules. *)
+stepping from a state with pc tag = Kernel, and that its own 
+cache lookups behave like the ground rules. *)
 
-Definition next_tr (mvec : MVec pvalue) : option pvalue :=
+Definition next_tpc_tr (mvec : MVec pvalue) : option (word mt * pvalue) :=
   do! opw <- known (cop mvec);
   do! opcode <- word_to_op opw;
+  let f (tpcp:pvalue) (trp:pvalue) :=
+      do! tpc <- known tpcp;
+      Some (tpc,trp) in
   match opcode with
-    | NOP => Some (C TNone)
-    | CONST => Some (C TKernel)
-    | MOV => Some (ct1 mvec)
-    | BINOP _ => Some (C TKernel)
-    | LOAD =>  Some (ct2 mvec)
-    | STORE => Some (ct2 mvec)
-    | JUMP => Some (C TNone)
-    | BNZ => Some (C TNone)
-    | JAL => Some (ctpc mvec)
-    | JUMPEPC => Some (C TNone)
-    | ADDRULE => Some (C TNone)
-    | GETTAG => Some (C TKernel)
-    | PUTTAG => Some (C TNone)
+    | NOP => f (ctpc mvec) (C TNone)
+    | CONST => f (ctpc mvec) (C TKernel)
+    | MOV => f (ctpc mvec) (ct1 mvec)
+    | BINOP _ => f (ctpc mvec) (C TKernel)
+    | LOAD =>  f (ctpc mvec) (ct2 mvec)
+    | STORE => f (ctpc mvec) (ct2 mvec)
+    | JUMP => f (ct1 mvec) (C TNone)
+    | BNZ => f (ctpc mvec) (C TNone)
+    | JAL => f (ct1 mvec) (ctpc mvec)
+    | JUMPEPC => f (ct1 mvec) (C TNone)
+    | ADDRULE => f (ctpc mvec) (C TNone)
+    | GETTAG => f (ctpc mvec) (C TKernel)
+    | PUTTAG => f (ctpc mvec) (C TNone)
     | HALT => None
     | SERVICE => None
   end.
 
 
 Definition next_pstate (mvec : MVec pvalue)
-                       (k : word mt -> pvalue -> option pstate) : option pstate :=
-  do! tr <- next_tr mvec;
-  k TKernel tr.
+                       (k : word mt  -> pvalue -> option pstate) : option pstate :=
+  do! tpc_tr : word mt*pvalue <- next_tpc_tr mvec;
+  let (tpc,tr) := tpc_tr in 
+  k tpc tr.
 
 Definition next_pstate_reg_and_pc (st : pstate) (mvec : MVec pvalue) r x pc' : option pstate :=
   next_pstate mvec (fun trpc tr =>
@@ -141,6 +152,29 @@ Variable masks: Masks.
    the PC and the instruction it points to precisely,
    (and, for memory operations, the precise address involved) *)
 
+Definition next_pstate_pc' st mvec v :=
+    do! t <- known(tag v);
+    match known (val v),is_kernel_tag t with
+      Some p,true =>
+        do! st' <- next_pstate_pc st mvec p;
+        Some (St st')
+    | None,false => 
+        Some UnknownUserSt
+    | _,_ => None
+    end.
+
+
+Definition next_pstate_reg_and_pc' st mvec ra x v  :=
+    do! t <- known(tag v);
+    match known (val v),is_kernel_tag t with
+      Some p,true =>
+        do! st' <- next_pstate_reg_and_pc st mvec ra x p;
+        Some (St st')
+    | None,false => 
+        Some UnknownUserSt 
+    | _,_ => None
+    end.
+  
 
 Definition pstep (st : pstate) : option tstate :=
   let 'mkPState mem reg cache pc@tpc epc := st in
@@ -194,9 +228,7 @@ Definition pstep (st : pstate) : option tstate :=
   | Jump r =>
     do! v <- PartMaps.get reg r;
     let mvec := mvec (tag v) (C TNone) (C TNone) in
-    do! pc' <- known (val v);
-    do! st' <- next_pstate_pc st mvec pc';
-    Some (St st')
+    next_pstate_pc' st mvec v
   | Bnz r n =>
     do! v <- PartMaps.get reg r;
     let mvec := mvec (tag v) (C TNone) (C TNone) in
@@ -207,10 +239,10 @@ Definition pstep (st : pstate) : option tstate :=
     do! v <- PartMaps.get reg r;
     do! old <- PartMaps.get reg ra;
     let mvec := mvec (tag v) (tag old) (C TNone) in
-    do! pc' <- known (val v);
-    do! st' <- next_pstate_reg_and_pc st mvec ra (C (pc.+1)) pc';
-    Some (St st')
-  | JumpEpc => None  (* For now at least, let's just say we can't do this. *)
+    next_pstate_reg_and_pc' st mvec ra (C (pc.+1)) v
+  | JumpEpc =>  
+    let mvec := mvec (tag epc) (C TNone) (C TNone) in
+    next_pstate_pc' st mvec epc
   | AddRule =>
     let mvec := mvec (C TNone) (C TNone) (C TNone) in
     do! st' <-
@@ -236,12 +268,14 @@ Definition pstep (st : pstate) : option tstate :=
          do! reg' <- PartMaps.upd reg r3 (val v1)@(val v2);
          Some (mkPState mem reg' cache (pc.+1)@trpc epc));
     Some (St st')
-  | Halt => None
+  | Halt => Some Halted
 end.
 
 
 Fixpoint tstep (ts: tstate) : option tstate :=
   match ts with
+  | Halted => Some Halted
+  | UnknownUserSt => Some UnknownUserSt
   | St s => pstep s
   | Ch z s1 s2 =>
       do! ts1 <- tstep s1;
@@ -277,6 +311,13 @@ Lemma concretize_known: forall pv w,
   concretize_pvalue pv = w.
 Proof.
   induction pv; intros; inv H; auto.
+  destruct (known pv1) eqn:?.
+  destruct (known pv2) eqn:?.
+  inv H1. 
+  erewrite <- (IHpv1 w0); auto.
+  erewrite <- (IHpv2 w1); auto. 
+  inv H1. 
+  inv H1. 
 Qed.
 
 Definition concretize_atom (a:patom) : atom :=
@@ -307,9 +348,11 @@ Definition concretize_pstate (ps:pstate) : state mt :=
           (concretize_atom (pepc ps)).
 
 
-Fixpoint concretize_tstate (ts:tstate) : state mt :=
+Fixpoint concretize_tstate (ts:tstate) : option (state mt) :=
   match ts with
-  | St ps => concretize_pstate ps
+  | Halted => None
+  | UnknownUserSt => None
+  | St ps => Some (concretize_pstate ps)
   | Ch z ts1 ts2 =>
         if concretize_pvalue z == Word.zero then
           concretize_tstate ts1
@@ -351,6 +394,8 @@ Ltac undo :=
                destruct t eqn:?; simpl in STEP; try discriminate
            | H : Some _ = Some _ |- _ =>
                inv H
+           | H : Some _ = None |- _ =>  discriminate
+           | H : None = Some |- _ =>  discriminate
          end.
 
 
@@ -358,46 +403,114 @@ Ltac undo :=
 
 Fixpoint kernel_tstate (ts: tstate mt) : Prop :=
   match ts with
+  | Halted => False (* ?? *)
+  | UnknownUserSt => False
   | St ps => tag (ppc mt ps) = TKernel 
   | Ch _ ts1 ts2 => kernel_tstate ts1 /\ kernel_tstate ts2
   end.
 
+Fixpoint normal_tstate (ts: tstate mt) : Prop :=
+  match ts with
+  | St _ => True
+  | Ch _ ts1 ts2 => normal_tstate ts1 /\ normal_tstate ts2
+  | _ => False
+  end.
+
+
 Lemma kernel_pstep: forall ps ts,
   tag (ppc mt ps) = TKernel  -> 
-  Some ts = pstep mt masks ps ->
+  Some ts = pstep mt masks ps -> normal_tstate ts -> 
   kernel_tstate ts.
 Proof.
   intros. unfold pstep in H0.  
   destruct ps.  simpl in H. subst. destruct ppc0. undo. 
-  destruct i; undo; try unfold next_pstate_pc in *;
-                    try unfold next_pstate_reg in *;
-                    try unfold next_pstate_reg_and_pc in *; 
-                    try unfold next_pstate in *; undo; simpl; auto. 
-  inv H0. 
-  inv H0. 
+  destruct i; 
+  undo; 
+  try unfold next_pstate_pc in *;
+  try unfold next_pstate_reg in *;
+  try unfold next_pstate_reg_and_pc in *; 
+  try unfold next_pstate in *; 
+  try unfold next_tpc_tr in *; 
+  undo; simpl in *; undo;
+  try match goal with 
+      H: word_to_op (op_to_word ?X) = Some _ |- _ => rewrite op_to_wordK in H; inv H
+  end; undo; auto.
+
+  try unfold next_pstate_pc' in *. undo. 
+  destruct (known mt (common.val a0)) eqn:?; undo; 
+  destruct (is_kernel_tag w0) eqn:?; undo.
+  try unfold next_pstate_pc in *;
+  try unfold next_pstate_reg in *;
+  try unfold next_pstate_reg_and_pc in *; 
+  try unfold next_pstate in *; 
+  try unfold next_tpc_tr in *; 
+  undo; simpl in *; undo;
+  try match goal with 
+      H: word_to_op (op_to_word ?X) = Some _ |- _ => rewrite op_to_wordK in H; inv H
+  end; undo; auto.
+  unfold is_kernel_tag in Heqb. simpl. 
+  have [eq|neq] := altP (w0 =P TKernel).  auto.
+  apply negb_true_iff in neq. rewrite neq in Heqb; discriminate.
+  inv H1. 
+
+  try unfold next_pstate_reg_and_pc' in *. undo. 
+  destruct (known mt (common.val a0)) eqn:?; undo; 
+  destruct (is_kernel_tag w0) eqn:?; undo.
+  try unfold next_pstate_pc in *;
+  try unfold next_pstate_reg in *;
+  try unfold next_pstate_reg_and_pc in *; 
+  try unfold next_pstate in *; 
+  try unfold next_tpc_tr in *; 
+  undo; simpl in *; undo;
+  try match goal with 
+      H: word_to_op (op_to_word ?X) = Some _ |- _ => rewrite op_to_wordK in H; inv H
+  end; undo; auto.
+  unfold is_kernel_tag in Heqb. simpl.
+  have [eq|neq] := altP (w0 =P TKernel).  auto.
+  apply negb_true_iff in neq. rewrite neq in Heqb; discriminate.
+  inv H1. 
+
+  try unfold next_pstate_pc' in *. undo. 
+  destruct (known mt (common.val pepc0)) eqn:?; undo; 
+  destruct (is_kernel_tag w0) eqn:?; undo.
+  try unfold next_pstate_pc in *;
+  try unfold next_pstate_reg in *;
+  try unfold next_pstate_reg_and_pc in *; 
+  try unfold next_pstate in *; 
+  try unfold next_tpc_tr in *; 
+  undo; simpl in *; undo;
+  try match goal with 
+      H: word_to_op (op_to_word ?X) = Some _ |- _ => rewrite op_to_wordK in H; inv H
+  end; undo; auto.
+  unfold is_kernel_tag in Heqb. simpl. 
+  have [eq|neq] := altP (w0 =P TKernel).  auto.
+  apply negb_true_iff in neq. rewrite neq in Heqb; discriminate.
+  inv H1. 
 Qed.
 
 Lemma kernel_tstep: forall ts ts',
   kernel_tstate ts -> 
-  Some ts' = tstep mt masks ts -> 
+  Some ts' = tstep mt masks ts -> normal_tstate ts' -> 
   kernel_tstate ts'. 
 Proof.
-  induction ts; intros. 
+  induction ts; intros.   
+  inv H0. inv H1. 
+  inv H0. inv H1.
   simpl in *. eapply kernel_pstep; eauto.
-  simpl in *. inv H. undo. 
+  simpl in *. inv H. undo. inv H1. 
   simpl; split; eauto.  
 Qed.
 
-(* parametric evaluation is sound *)
+(* parametric evaluation is sound in the three cases of interest *)
 
-Hypothesis sound_next_tr : forall env cache (mvec: MVec (pvalue mt)) (tr:pvalue mt),
+Hypothesis sound_next_tpc_tr : forall env cache (mvec: MVec (pvalue mt)) (tpc:word mt) (tr:pvalue mt),
   ctpc mvec = C mt TKernel ->
-  Some tr = next_tr mt mvec ->
-  Some (mkRVec TKernel (concretize_pvalue mt env tr)) = cache_lookup cache masks (concretize_mvec mt env mvec).
+  Some (tpc,tr) = next_tpc_tr mt mvec ->
+  Some (mkRVec tpc (concretize_pvalue mt env tr)) = cache_lookup cache masks (concretize_mvec mt env mvec).
 
 Lemma sound_next_pstate : forall env ps mvec k kk ps',
   ctpc mvec = C mt TKernel ->
-  (forall tr ps', Some ps' = k TKernel tr -> Some (concretize_pstate mt env ps') = kk (mkRVec TKernel (concretize_pvalue mt env tr))) ->
+  (forall tpc tr ps', Some ps' = k tpc  tr -> Some (concretize_pstate mt env ps') = kk (mkRVec tpc (concretize_pvalue mt env tr))) ->
   Some ps' = next_pstate mt mvec k ->
   Some (concretize_pstate mt env ps') = next_state masks (concretize_pstate mt env ps) (concretize_mvec mt env mvec) kk.
 Proof.
@@ -405,13 +518,15 @@ Proof.
   unfold next_state.
   unfold next_pstate in H1.
   undo.
-  erewrite <- sound_next_tr.
-  3: rewrite Heqo; auto.
+  destruct p. 
+  erewrite <- sound_next_tpc_tr.
+  3: rewrite Heqo; eauto.
   erewrite <- H0.
-  2: rewrite <- H1; auto.
+  eauto.
   auto.
   auto.
 Qed.
+
 
 Lemma sound_add_rule: forall env
                              (pcache pcache' : rules (pvalue mt))
@@ -441,7 +556,7 @@ Proof.
 Qed.
 
 Lemma sound_next_pstate_reg_and_pc: forall env ps mvec r x pc' ps',
-  ctpc mvec = C mt TKernel ->
+  ctpc mvec = C mt TKernel -> 
   Some ps' = next_pstate_reg_and_pc mt ps mvec r x pc' ->
   Some (concretize_pstate mt env ps') = next_state_reg_and_pc masks (concretize_pstate mt env ps) (concretize_mvec mt env mvec) r (concretize_pvalue mt env x) pc'.
 Proof.
@@ -459,6 +574,7 @@ Proof.
   erewrite PartMaps.map_upd; eauto. simpl.
   auto.
 Qed.
+
 
 Lemma sound_next_pstate_reg: forall env ps mvec r x ps',
   ctpc mvec = C mt TKernel ->
@@ -482,11 +598,13 @@ Proof.
   auto.
 Qed.
 
+(* First case: a normal step *)
 
-Lemma sound_step : forall env ps ts,
+Lemma sound_normal_step : forall env ps ts,
   tag (ppc mt ps) = TKernel ->
+  forall NS: normal_tstate ts,
   Some ts = pstep mt masks ps ->
-  Some (concretize_tstate mt env ts) = step masks mt (concretize_pstate mt env ps).
+  concretize_tstate mt env ts = step masks mt (concretize_pstate mt env ps).
 Proof.
   intros.
   unfold step. (* unfold concretize_pstate.  *)
@@ -503,27 +621,32 @@ Proof.
   rewrite Heqo1.  simpl.
   destruct i.
 
+  (* Nop *)
   undo.
   simpl.
   symmetry in Heqo2.
   erewrite (sound_next_pstate_pc _ _ _ _ _ _ Heqo2); eauto.
 
+  (* Const *)
   undo.
   rewrite PartMaps.map_correctness. rewrite Heqo2. simpl.
   symmetry in Heqo3.
   erewrite (sound_next_pstate_reg _ _ _ _ _ _ _ Heqo3); eauto.
 
+  (* Mov *)
   undo.
   repeat rewrite PartMaps.map_correctness. rewrite Heqo2. rewrite Heqo3. simpl.
   symmetry in Heqo4.
   erewrite (sound_next_pstate_reg _ _ _ _ _ _ _ Heqo4); eauto.
 
+  (* Binop *)
   undo.
   repeat rewrite PartMaps.map_correctness.
   rewrite Heqo2. rewrite Heqo3. rewrite Heqo4. simpl.
   symmetry in Heqo5.
   erewrite (sound_next_pstate_reg _ _ _ _ _ _ _ Heqo5); eauto.
 
+  (* Load *)
   undo.
   repeat rewrite PartMaps.map_correctness.
   rewrite Heqo2. simpl. rewrite (concretize_known _ env _ _ Heqo3).
@@ -532,6 +655,7 @@ Proof.
   symmetry in Heqo6.
   erewrite (sound_next_pstate_reg _ _ _ _ _ _ _ Heqo6); eauto.
 
+  (* Store *)
   undo.
   repeat rewrite PartMaps.map_correctness.
   rewrite Heqo2. rewrite Heqo3. simpl.
@@ -562,13 +686,22 @@ Proof.
   erewrite PartMaps.map_upd; eauto.
   simpl. auto.
 
+  (* Jump *)
   undo.
   repeat rewrite PartMaps.map_correctness.
   rewrite Heqo2. simpl.
-  rewrite (concretize_known _ env _ _ Heqo3).
-  symmetry in Heqo4.
-  erewrite (sound_next_pstate_pc _ _ _ _ _ _ Heqo4); eauto.
+  unfold next_pstate_pc' in H0. undo. 
+  destruct (known mt (common.val a0)) eqn:?;
+  destruct (is_kernel_tag w0) eqn:?; try discriminate. 
+  undo.
+  simpl. 
+  rewrite (concretize_known _ env _ _ Heqo4).
+  symmetry in Heqo5.
+  erewrite (sound_next_pstate_pc _ _ _ _ _ _ Heqo5); eauto.
+  undo.
+  inv NS. 
 
+  (* Bnz *)
   undo.
   repeat rewrite PartMaps.map_correctness.
   rewrite Heqo2. simpl.
@@ -578,15 +711,34 @@ Proof.
   symmetry in Heqo4.
   erewrite (sound_next_pstate_pc _ _ _ _ _ _ Heqo4); eauto.
 
+  (* Jal *)
   undo.
   repeat rewrite PartMaps.map_correctness.
   rewrite Heqo2. rewrite Heqo3. simpl.
-  rewrite (concretize_known _ env _ _ Heqo4).
-  symmetry in Heqo5.
-  erewrite (sound_next_pstate_reg_and_pc _ _ _ _ _ _ _ _ Heqo5); eauto.
+  unfold next_pstate_reg_and_pc' in H0.  undo. 
+  destruct (known mt (common.val a0)) eqn:?;
+  destruct (is_kernel_tag w0) eqn:?; try discriminate. 
+  undo.
+  simpl. 
+  rewrite (concretize_known _ env _ _ Heqo5).
+  symmetry in Heqo6.
+  erewrite (sound_next_pstate_reg_and_pc _ _ _ _ _ _ _ _ Heqo6); eauto.
+  undo. inv NS. 
 
-  undo. discriminate.
 
+  (* JumpEPC *)
+  unfold next_pstate_pc' in H0. undo.
+  destruct (known mt (common.val pepc0)) eqn:?;
+  destruct (is_kernel_tag w0) eqn:?; try discriminate. 
+  undo.
+  simpl.
+  rewrite (concretize_known _ env _ _ Heqo3). 
+  symmetry in Heqo4. 
+  erewrite (sound_next_pstate_pc _ _ _ _ _ _ Heqo4); eauto.
+  undo. inv NS. 
+
+
+  (* AddRule *)
   undo. simpl.
   replace
    ({|
@@ -611,12 +763,14 @@ Proof.
   erewrite sound_add_rule; eauto.
   simpl.  auto.
 
+  (* GetTag *)
   undo.
   repeat rewrite PartMaps.map_correctness.
   rewrite Heqo2.  rewrite Heqo3. simpl.
   symmetry in Heqo4.
   erewrite (sound_next_pstate_reg _ _ _ _ _ _ _ Heqo4); eauto.
 
+  (* PutTag *)
   undo.
   repeat rewrite PartMaps.map_correctness.
   rewrite Heqo2.  rewrite Heqo3. rewrite Heqo4. simpl.
@@ -647,7 +801,9 @@ Proof.
   erewrite PartMaps.map_upd; eauto.
   auto.
 
-  discriminate.
+  (* Halt *)
+  inv H0. inv NS.
+
 
   Grab Existential Variables. (* ??? !!! *)
 
@@ -660,33 +816,166 @@ Proof.
   reflexivity.
   reflexivity.
   reflexivity.
-  reflexivity.
+  reflexivity. 
+  reflexivity. 
 Qed.
 
-Lemma sound_tstep: forall env ts ts',
+
+(* Second case: a step back to user mode. 
+   There should be a matching step  *)
+
+Lemma sound_unknown_user_step : forall env ps,
+  tag (ppc mt ps) = TKernel ->
+  Some (UnknownUserSt mt) = pstep mt masks ps ->
+  exists (s:state mt),
+  Some s = step masks mt (concretize_pstate mt env ps)
+  /\ not (is_kernel_tag (tag (pc s))).
+
+Proof.
+  intros.
+  unfold step. (* unfold concretize_pstate.  *)
+  unfold pstep in H0.
+  destruct ps. simpl.
+  destruct ppc0.
+  simpl in H. subst tag.
+  undo.
+  replace (PartMaps.get (PartMaps.map (concretize_atom mt env) pmem0) val)
+          with (option_map (concretize_atom mt env) (PartMaps.get pmem0 val))
+                 by (rewrite <- PartMaps.map_correctness; auto).
+  rewrite Heqo.  simpl.
+  rewrite (concretize_known _ env _ _ Heqo0).
+  rewrite Heqo1.  simpl.
+  destruct i; undo.
+
+  (* Jump *)
+  undo.
+  repeat rewrite PartMaps.map_correctness.
+  rewrite Heqo2. simpl.
+  unfold next_pstate_pc' in H0. undo. 
+  destruct (known mt (common.val a0)) eqn:?;
+  destruct (is_kernel_tag w0) eqn:?; try discriminate. 
+  undo.
+  rewrite (concretize_known _ env _ _ Heqo3). 
+  eexists. 
+  split.
+  replace
+   ({|
+    cop := op_to_word JUMP;
+    ctpc := TKernel;
+    cti := concretize_pvalue mt env (tag a);
+    ct1 := w0;
+    ct2 := TNone;
+    ct3 := TNone |})
+   with
+    (concretize_mvec mt env
+       {|
+         cop := (C mt (op_to_word JUMP));
+         ctpc := (C mt TKernel);
+         cti := tag a;
+         ct1 := (C mt w0);
+         ct2 := (C mt TNone);
+         ct3 := (C mt TNone) |}) by auto.  (* why is this needed? *)
+  eapply sound_next_pstate_pc. 
+  auto.
+  unfold next_pstate_pc. simpl. 
+  unfold next_pstate. unfold next_tpc_tr. simpl. 
+  rewrite op_to_wordK. simpl.  eauto.
+  simpl. rewrite Heqb. auto. 
+
+  (* Jal *)
+  admit. (* similar *)
+
+  (* JumpEPC *)
+  admit. (* similar *)
+Qed.
+
+
+(* Third case: a step to Halted.
+   There should be no step at all. 
+   Could combine this statement with the normal case. *)
+
+Set Printing Depth 20.
+
+Lemma sound_halt_step : forall env ps,
+  Some (Halted mt) = pstep mt masks ps ->
+  None = step masks mt (concretize_pstate mt env ps).
+Proof.
+  intros.
+  unfold step. (* unfold concretize_pstate.  *)
+  unfold pstep in H.
+  destruct ps. simpl.
+  destruct ppc0.
+  undo.
+  replace (PartMaps.get (PartMaps.map (concretize_atom mt env) pmem0) val)
+          with (option_map (concretize_atom mt env) (PartMaps.get pmem0 val))
+                 by (rewrite <- PartMaps.map_correctness; auto).
+  rewrite Heqo.  simpl.
+  rewrite (concretize_known _ env _ _ Heqo0).
+  rewrite Heqo1.  simpl.
+  destruct i; undo.
+
+  (* Jump *)
+  unfold next_pstate_pc' in H; undo.
+  destruct (known mt (common.val a0)) eqn:?;
+  destruct (is_kernel_tag w0) eqn:?; try discriminate. 
+  undo.
+  undo.
+
+  (* Jal *)
+  unfold next_pstate_reg_and_pc' in H;  undo. 
+  destruct (known mt (common.val a0)) eqn:?;
+  destruct (is_kernel_tag w0) eqn:?; try discriminate. 
+  undo.
+  undo.
+
+  (* JumpEpc *)
+  unfold next_pstate_pc' in H; undo.
+  destruct (known mt (common.val pepc0)) eqn:?;
+  destruct (is_kernel_tag w0) eqn:?; try discriminate. 
+  undo.
+  undo.
+  
+  (* Halt *)
+  auto.
+Qed.
+
+(* Not sure if this particular form is still useful.. -- too weak *)
+Lemma sound_tstep: forall env ts ts' s,
   kernel_tstate ts -> 
+  forall NS: normal_tstate ts',
   Some ts' = tstep mt masks ts ->
-  Some (concretize_tstate mt env ts') = step masks mt (concretize_tstate mt env ts).
+  Some s = concretize_tstate mt env ts -> 
+  concretize_tstate mt env ts' = step masks mt s.
 Proof.
   induction ts; intros. 
-    inv H. eapply sound_step; eauto. 
-    inv H0. undo. inv H. 
+    inv H. 
+    inv H. 
+    inv H. destruct (concretize_tstate mt env (St mt p)) eqn:?.
+      inv H1.  inv Heqo. eapply sound_normal_step; eauto. 
+      inv H1. 
+    inv H0. undo. simpl in H1. inv H. inv NS. 
     simpl. 
+    generalize H1. 
     have [zer|nonzer] := altP (concretize_pvalue mt env p =P Word.zero); eauto.
 Qed.    
 
-Lemma sound_eval : forall env fuel ts ts', 
+(* Not right...
+
+Lemma sound_eval : forall env fuel ts ts' s, 
   kernel_tstate ts -> 
   Some ts' = teval mt masks fuel ts -> 
-  Some (concretize_tstate mt env ts') = eval fuel (concretize_tstate mt env ts). 
+  kernel_tstate ts' -> 
+  Some s = concretize_tstate mt env ts -> 
+  concretize_tstate mt env ts' = eval fuel s.
 Proof.
   induction fuel; intros. 
     inv H0. auto.
     simpl. simpl in H0. undo. 
     symmetry in Heqo. 
-    erewrite <- sound_tstep; eauto. simpl. 
+    erewrite <- sound_tstep; eauto. . simpl. 
     eapply IHfuel; eauto. 
     eapply kernel_tstep; eauto.
 Qed. 
+*)
 
 End WithStuff.
